Defined eval_mexpr

coq-osiris/theories/semantics/eval.v
@@ -1,6 +1,7 @@
 From osiris Require Import base.
 From osiris.lang Require Import lang.
 From osiris.semantics Require Import code.
+From Equations Require Import Equations.
 Local Infix "=?" := String.eqb.
 
 (* Conventional metavariables. *)
@@ -9,22 +10,22 @@ Implicit Type g x : var.
 Implicit Type c : data. (* or coercion; TODO *)
 Implicit Type f : field.
 Implicit Type p : pat.
-Implicit Type ps : pats.
+Implicit Type ps : list pat.
 Implicit Type e : expr.
-Implicit Type es : exprs.
-Implicit Type fes : fexprs.
+Implicit Type es : list expr.
+Implicit Type fes : list fexpr.
 Implicit Type a : anonfun.
 Implicit Type v : val.
-Implicit Type vs : vals.
+Implicit Type vs : list val.
 Implicit Type fvs xvs : env.
 Implicit Type η δ : env.
-Implicit Type rbs : rec_bindings.
+Implicit Type rbs : list rec_binding.
 Implicit Type i : int.
 Implicit Type M : module.
 Implicit Type π : path.
 Implicit Type me : mexpr.
 Implicit Type item : sitem.
-Implicit Type items : sitems.
+Implicit Type items : list sitem.
 
 (* ------------------------------------------------------------------------ *)
 (* ------------------------------------------------------------------------ *)
@@ -78,7 +79,7 @@ Definition type_mismatch {A} (msg : string) : micro A :=
 (* [ok] is an inert computation. It produces the value [VUnit]. *)
 
 Notation ok :=
-  (ret (VData "()" $ VTuple VNil)).
+  (ret (VData "()" $ VTuple [])).
 
 (* ------------------------------------------------------------------------ *)
 (* ------------------------------------------------------------------------ *)
@@ -183,9 +184,9 @@ Definition as_struct (m : micro val) : micro env :=
 
 Fixpoint lookup_name η x : micro val :=
   match η with
-  | EnvCons x' v η =>
+  | (x', v) :: η =>
       if x =? x' then ret v else lookup_name η x
-  | EnvNil =>
+  | [] =>
       missing_variable_or_field x
   end.
 
@@ -206,30 +207,17 @@ Fixpoint lookup_path η π : micro val :=
 
 (* ------------------------------------------------------------------------ *)
 
-(* [concat δ η] concatenates the environment fragment [δ] in front of the
-   environment [η], yielding an extended environment. *)
-
-Fixpoint concat δ η : env :=
-  match δ with
-  | EnvNil =>
-      η
-  | EnvCons x v δ =>
-      EnvCons x v (concat δ η)
-  end.
-
-(* ------------------------------------------------------------------------ *)
-
 (* [remove f fvs] removes field [f] from the field-value list [fvs]. *)
 
 Fixpoint remove f fvs : micro env :=
   match fvs with
-  | EnvCons f' v fvs =>
+  | (f', v) :: fvs =>
       if f =? f' then
         ret fvs
       else
         fvs ← remove f fvs ;
-        ret (EnvCons f' v fvs)
-  | EnvNil =>
+        ret ((f', v) :: fvs)
+  | [] =>
       missing_field f
   end.
 
@@ -240,11 +228,11 @@ Fixpoint remove f fvs : micro env :=
 
 Fixpoint update fvs fvs' : micro env :=
   match fvs' with
-  | EnvNil =>
+  | [] =>
       ret fvs
-  | EnvCons f v' fvs' =>
+  | (f, v') :: fvs' =>
       fvs ← remove f fvs ;
-      let fvs := EnvCons f v' fvs in
+      let fvs := (f, v') :: fvs in
       update fvs fvs'
   end.
 
@@ -270,22 +258,16 @@ End StringOrder.
 
 Module StringSort := Sort StringOrder.
 
-Fixpoint domain (η : env) : list string :=
-  match η with
-  | EnvNil =>
-      []
-  | EnvCons x v η =>
-      x :: domain η
-  end.
+Definition domain (η : env) : list string := fst (split η).
 
 Fixpoint build (η : env) (xs : list string) : micro env :=
   match xs with
   | [] =>
-      ret EnvNil
+      ret []
   | x :: xs =>
       v ← lookup_name η x ;
       xs ← build η xs ;
-      ret (EnvCons x v xs)
+      ret ((x, v) :: xs)
   end.
 
 Definition sort (η : env) : micro env :=
@@ -303,10 +285,10 @@ Definition sort (η : env) : micro env :=
 
 Fixpoint eval_rec_bindings_aux η rbs rbs' : env :=
   match rbs' with
-  | RecBiNil =>
-      EnvNil
-  | RecBiCons (RecBinding g _a) rbs' =>
-      EnvCons g (VCloRec η rbs g) (eval_rec_bindings_aux η rbs rbs')
+  | [] =>
+      []
+  | (RecBinding g _a) :: rbs' =>
+      (g, (VCloRec η rbs g)) :: (eval_rec_bindings_aux η rbs rbs')
   end.
 
 (* [eval_rec_bindings η rbs] transforms the bindings [rbs] into an environment
@@ -323,9 +305,9 @@ Definition eval_rec_bindings η rbs : env :=
 
 Fixpoint lookup_rec_bindings rbs g : micro anonfun :=
   match rbs with
-  | RecBiCons (RecBinding g' a) rbs =>
+  | (RecBinding g' a) :: rbs =>
       if g =? g' then ret a else lookup_rec_bindings rbs g
-  | RecBiNil =>
+  | [] =>
       missing_variable g
   end.
 
@@ -357,20 +339,42 @@ Fixpoint extend δ p v : micro env :=
   | PVar x, _ =>
       (* A variable pattern always succeeds, and causes the environment
          to be extended. *)
-      ret (EnvCons x v δ)
+      ret ((x, v) :: δ)
   | PAlias p x, _ =>
       (* An alias pattern [p as x] is an intersection pattern: the value
          [v] must match both the pattern [p] and the pattern [x]. *)
       δ ← extend δ p v ;
-      ret (EnvCons x v δ)
+      ret ((x, v) :: δ)
   | POr p1 p2, _ =>
       (* A disjunction pattern [p1 | p2] requires that the value [v]
          match either [p1] or [p2]. *)
       orelse (extend δ p1 v) (extend δ p2 v)
   | PTuple ps, VTuple vs =>
       (* A tuple pattern matches a tuple value. *)
-      (* A hard failure occurs when [length ps ≠ length vs]. *)
-      extends δ ps vs
+
+      (* [extends δ ps vs] matches the values [vs] against the patterns [ps].
+         In case of success, the result is an extension of the environment
+         fragment [δ] with bindings for the bound variables of the patterns [ps].
+
+         A hard failure occurs when [length ps ≠ length vs]. *)
+
+      (* Pattern matching is sequential and obeys a left-to-right strategy. This
+         is important in the presence of GADTs, as the success of a test in the
+         left-hand side of a pair can guarantee the safety of a test in the
+         right-hand side of this pair. *)
+      ((fix extends (δ : env) ps vs : micro env :=
+        match ps, vs with
+        | [], [] =>
+            ret δ
+        | p::ps, v::vs =>
+            δ ← extend δ p v ;
+            δ ← extends δ ps vs ;
+            ret δ
+        | _::_, [] =>
+            length_mismatch "longer tuple expected"
+        | [], _::_ =>
+            length_mismatch "shorter tuple expected"
+        end) δ ps vs)
   | PData c p, VData c' v =>
       (* A data pattern matches a data value, provided the data constructors
          match. If the data constructors do not match, a soft failure takes
@@ -379,9 +383,26 @@ Fixpoint extend δ p v : micro env :=
   | PRecord fps, VRecord fvs =>
       (* A record pattern matches a record value. *)
       (* The pattern may have fewer fields than the value. *)
-      (* A hard failure occurs if a field is present in the pattern
-         but absent in the value. *)
-      extendfs δ fps fvs
+
+      (* [extendfs δ fps fvs] matches the field-indexed values [fvs] against the
+         field-indexed patterns [fps].
+
+         In case of success, the result is an extension of the environment
+         fragment [δ] with bindings for the bound variables of
+         the patterns [fps].
+
+         A hard failure occurs if a field is present in [fps]
+         but absent in [fvs]. *)
+      ((fix extendfs (δ : env) fps fvs : micro env :=
+          match fps with
+          | [] =>
+              ret δ
+          | (f, p)::fps =>
+              v ← lookup_name fvs f ;
+              δ ← extend δ p v ;
+              δ ← extendfs δ fps fvs ;
+              ret δ
+        end) δ fps fvs)
   | PInt z, VInt i' =>
       let i := int.repr z in
       if int.eq i i' then ret δ else next
@@ -401,52 +422,7 @@ Fixpoint extend δ p v : micro env :=
       type_mismatch "char expected"
   | PString _, _ =>
       type_mismatch "string expected"
-end
-
-(* [extends δ ps vs] matches the values [vs] against the patterns [ps].
-
-   In case of success, the result is an extension of the environment
-   fragment [δ] with bindings for the bound variables of the patterns [ps].
-
-   A hard failure occurs when [length ps ≠ length vs]. *)
-
-(* Pattern matching is sequential and obeys a left-to-right strategy. This
-   is important in the presence of GADTs, as the success of a test in the
-   left-hand side of a pair can guarantee the safety of a test in the
-   right-hand side of this pair. *)
-
-with extends δ ps vs : micro env :=
-  match ps, vs with
-  | PNil, VNil =>
-      ret δ
-  | PCons p ps, VCons v vs =>
-      δ ← extend δ p v ;
-      δ ← extends δ ps vs ;
-      ret δ
-  | PCons _ _, VNil =>
-      length_mismatch "longer tuple expected"
-  | PNil, VCons _ _ =>
-      length_mismatch "shorter tuple expected"
-  end
-
-(* [extendfs δ fps fvs] matches the field-indexed values [fvs] against the
-   field-indexed patterns [fps].
-
-   In case of success, the result is an extension of the environment fragment
-   [δ] with bindings for the bound variables of the patterns [fps].
-
-   A hard failure occurs if a field is present in [fps] but absent in [fvs]. *)
-
-with extendfs δ fps fvs : micro env :=
-  match fps with
-  | FPNil =>
-      ret δ
-  | FPCons f p fps =>
-      v ← lookup_name fvs f ;
-      δ ← extend δ p v ;
-      δ ← extendfs δ fps fvs ;
-      ret δ
-  end.
+end.
 
 (* ------------------------------------------------------------------------ *)
 
@@ -458,7 +434,7 @@ Definition acall η a v : micro val :=
   let '(AnonFun x e) := a in
   (* Extend the environment [η] with a binding of the variable [x]
      to the value [v]. *)
-  let η := EnvCons x v η in
+  let η := (x, v) :: η in
   (* Then, evaluate the function body [e]. A recursive call to [eval] cannot
      be used, so evaluation of [e] is requested via a [stop] effect. *)
   stop CEval (η, e).
@@ -477,7 +453,7 @@ Definition call v1 v2 : micro val :=
       (* Extend the environment [η] found in the closure with bindings
          for the recursive functions in [rbs]. *)
       let δ := eval_rec_bindings η rbs in
-      let η := concat δ η in
+      let η := δ ++ η in
       (* Look up the entry point [g] in [rbs], yielding an anonymous
          function [a]. *)
       a ← lookup_rec_bindings rbs g ;
@@ -518,27 +494,25 @@ Fixpoint eq_val v1 v2 : micro bool :=
   | VString s1, VString s2 =>
       ret (s1 =? s2)
   | VTuple vs1, VTuple vs2 =>
-      eq_vals vs1 vs2
+      ((fix eq_vals vs1 vs2 :=
+        match vs1, vs2 with
+        | [], [] =>
+            ret true
+        | v1 :: vs1, v2 :: vs2 =>
+            b ← eq_val v1 v2 ;
+            b' ← eq_vals vs1 vs2 ;
+            ret (b && b')
+        |  _ :: _, []
+        | [], _ :: _ =>
+            structural_equality_error "tuple length mismatch"
+        end) vs1 vs2)
   | VData c1 v1, VData c2 v2 =>
       let b := c1 =? c2 in
       b' ← eq_val v1 v2 ;
       ret (b && b')
   | _, _ =>
       structural_equality_error "invalid or unsupported arguments"
-  end
-
-with eq_vals vs1 vs2 : micro bool :=
-  match vs1, vs2 with
-  | VNil, VNil =>
-      ret true
-  | VCons v1 vs1, VCons v2 vs2 =>
-      b ← eq_val v1 v2 ;
-      b' ← eq_vals vs1 vs2 ;
-      ret (b && b')
-  | VCons _ _, VNil
-  | VNil, VCons _ _ =>
-      structural_equality_error "tuple length mismatch"
-  end.
+end.
 
 Definition ne_val v1 v2 :=
   b ← eq_val v1 v2 ;
@@ -602,7 +576,7 @@ Definition ge_val v1 v2 :=
    [acall]) and when the body of a loop is executed (see [loop]). *)
 
 Definition ret_concat δ η : micro env :=
-  ret (concat δ η).
+  ret (δ ++ η).
 
 (* ------------------------------------------------------------------------ *)
 
@@ -625,7 +599,7 @@ Implicit Type ηδ : envs.
 
 Definition dconcat δ' ηδ : envs :=
   let '(η, δ) := ηδ in
-  (concat δ' η, concat δ' δ).
+  (δ' ++ η, δ' ++ δ).
 
 (* TODO comment *)
 
@@ -646,31 +620,25 @@ Fixpoint coerce (c : coercion) (v : val) : micro val :=
       xvs ← val_as_struct v ;
       (* From [xvs], fetch the components named in the list [xcs], and
          apply the corresponding coercions to them. *)
-      xvs ← coerces xcs xvs ;
-      (* Return a structure. *)
-      ret (VStruct xvs)
-  end
-
-(* [coerces xcs xvs] applies the name-coercion list [xcs] to the
-   name-value list [xvs], producing a new name-value list. *)
-
-with coerces (xcs : fcoercions) (xvs : env) : micro env :=
-  match xcs with
-  | CNil =>
-      ret EnvNil
-  | CCons x c xcs =>
-      (* Fetch the component [x] from [xvs]. *)
-      v ← lookup_name xvs x ;
-      (* Apply the coercion [c] to it. *)
-      v ← coerce c v ;
-      (* Fetch the rest. *)
-      xvs ← coerces xcs xvs ;
-      (* Combine the results. Whether we place [x] in front of [xvs] or
-         behind [xvs] should not make any difference, because the field
-         names that appear in the coercion should be pairwise distinct,
-         so the order in which these fields appear in the new structure
-         should be irrelevant. *)
-      ret (EnvCons x v xvs)
+      bind ((fix coerces (xcs : list fcoercion ) xvs : micro env :=
+             match xcs with
+             | [] =>
+                 ret []
+             | (x, c) :: xcs =>
+                 (* Fetch the component [x] from [xvs]. *)
+                 v ← lookup_name xvs x ;
+                 (* Apply the coercion [c] to it. *)
+                 v ← coerce c v ;
+                 (* Fetch the rest. *)
+                 xvs ← coerces xcs xvs ;
+                 (* Combine the results. Whether we place [x] in front of [xvs] or
+                    behind [xvs] should not make any difference, because the field
+                    names that appear in the coercion should be pairwise distinct,
+                    so the order in which these fields appear in the new structure
+                    should be irrelevant. *)
+                 ret ((x, v) :: xvs)
+             end) xcs xvs)
+      (λ xvs : env, ret (VStruct xvs))
   end.
 
 (* ------------------------------------------------------------------------ *)
@@ -700,342 +668,731 @@ with coerces (xcs : fcoercions) (xvs : env) : micro env :=
    these expressions is possible: the evaluation order is not necessarily
    left-to-right or right-to-left. *)
 
-Fixpoint eval η e : micro val :=
+Open Scope nat.
+Fixpoint length_expr (e : expr) : nat :=
   match e with
-  | EUnsupported =>
-      unsupported_construct
-  | EChar c =>
-      ret (VChar c)
-  | EPath π =>
-      (* A path [π] is looked up in the environment [η]. *)
-      lookup_path η π
-  | EAnonFun a =>
-      (* The creation of a closure captures the environment [η]. *)
-      (* This environment is *not* trimmed so as to keep only the variables
-         that occur free in [a]. Indeed, in OCaml, due to [open], [include]
-         and other constructs, it is not easy to statically compute the set
-         of free variables of an expression. *)
-      ret (VClo η a)
-  | EApp e1 e2 =>
-      (* The expressions [e1] and [e2] are evaluated in parallel. *)
-      '(v1, v2) ← par (eval η e1) (eval η e2) ;
-      call v1 v2
-  | ETuple es =>
-      (* The tuple components are evaluated in parallel. *)
-      vs ← evals η es ;
-      ret (VTuple vs)
-  | EData c e =>
-      v ← eval η e ;
-      ret (VData c v)
-  | ERecord fes =>
-      (* The record components are evaluated in parallel. *)
-      fvs ← evalfs η fes ;
-      fvs ← sort fvs ;
-      ret (VRecord fvs)
-  | ERecordUpdate e fes =>
-      (* The existing record and the new record components are evaluated in
-         parallel. *)
-      '(fvs, fvs') ← par (as_record (eval η e)) (evalfs η fes) ;
-      (* The new components override existing components by the same name. *)
-      fvs ← update fvs fvs' ;
-      fvs ← sort fvs ;
-      ret (VRecord fvs)
-  | ERecordAccess e f =>
-      fvs ← as_record (eval η e) ;
-      lookup_name fvs f
-  | EBoolConj e1 e2 =>
-      b1 ← as_bool (eval η e1) ;
-      if (b1 : bool) then eval η e2 else ret VFalse
-  | EString s =>
-      ret (VString s)
-  | EInt i =>
-      (* An integer literal is interpreted as a machine integer. *)
-      (* We do not require this integer literal to lie within a certain
-         range; we project it into the range of machine integers. *)
-      ret (VInt (int.repr i))
-  | EMaxInt =>
-      ret (VInt (int.repr int.max_signed))
-  | EMinInt =>
-      ret (VInt (int.repr int.min_signed))
-  | EIntNeg e =>
-      i ← as_int (eval η e) ;
-      ret (VInt (int.neg i))
-  | EIntAdd e1 e2 =>
-      '(i1, i2) ← par (as_int (eval η e1)) (as_int (eval η e2)) ;
-      ret (VInt (int.add i1 i2))
-  | EIntSub e1 e2 =>
-      '(i1, i2) ← par (as_int (eval η e1)) (as_int (eval η e2)) ;
-      ret (VInt (int.sub i1 i2))
-  | EIntMul e1 e2 =>
-      '(i1, i2) ← par (as_int (eval η e1)) (as_int (eval η e2)) ;
-      ret (VInt (int.mul i1 i2))
-  | EIntDiv e1 e2 =>
-      (* Signed division is used. *)
-      '(i1, i2) ← par (as_int (eval η e1)) (as_int (eval η e2)) ;
-      '() ← check_div_by_zero i2 ;
-      ret (VInt (int.divs i1 i2))
-  | EIntMod e1 e2 =>
-      (* Signed remainder is used. *)
-      '(i1, i2) ← par (as_int (eval η e1)) (as_int (eval η e2)) ;
-      '() ← check_div_by_zero i2 ;
-      ret (VInt (int.mods i1 i2))
-  | EOpPhysEq e1 e2 =>
-      '(v1, v2) ← par (eval η e1) (eval η e2) ;
-      b ← phys_eq_val v1 v2 ;
-      ret (VBool b)
-  | EOpEq e1 e2 =>
-      '(v1, v2) ← par (eval η e1) (eval η e2) ;
-      b ← eq_val v1 v2 ;
-      ret (VBool b)
-  | EOpNe e1 e2 =>
-      '(v1, v2) ← par (eval η e1) (eval η e2) ;
-      b ← ne_val v1 v2 ;
-      ret (VBool b)
-  | EOpLt e1 e2 =>
-      '(v1, v2) ← par (eval η e1) (eval η e2) ;
-      b ← lt_val v1 v2 ;
-      ret (VBool b)
-  | EOpLe e1 e2 =>
-      '(v1, v2) ← par (eval η e1) (eval η e2) ;
-      b ← le_val v1 v2 ;
-      ret (VBool b)
-  | EOpGt e1 e2 =>
-      '(v1, v2) ← par (eval η e1) (eval η e2) ;
-      b ← gt_val v1 v2 ;
-      ret (VBool b)
-  | EOpGe e1 e2 =>
-      '(v1, v2) ← par (eval η e1) (eval η e2) ;
-      b ← ge_val v1 v2 ;
-      ret (VBool b)
-  | EBoolDisj e1 e2 =>
-      b1 ← as_bool (eval η e1) ;
-      if (b1 : bool) then ret VTrue else eval η e2
-  | EBoolNeg e =>
-      b ← as_bool (eval η e) ;
-      ret (VBool (negb b))
+  | EUnsupported => 1
+  | EPath _ => 1
+  | EAnonFun afun =>
+      match afun with
+      | AnonFun _ e => 1 + length_expr e end
+  | EApp e1 e2 => 1 + length_expr e1 + length_expr e2
+  | ETuple es => fold_left (fun acc e => (length_expr e) + acc) es 1
+  | EData _ e => 1 + length_expr e
+  | ERecord fexprs =>
+      fold_left (fun acc fe =>
+                   match fe with
+                   | Fexpr _ e =>
+                       (length_expr e) + acc
+                   end) fexprs 1
+  | ERecordUpdate e fexprs =>
+      fold_left (fun acc fe =>
+                   match fe with
+                   | Fexpr _ e =>
+                       (length_expr e) + acc
+                   end) fexprs (1 + length_expr e)
+  | ERecordAccess e _ => 1 + length_expr e
+  | EBoolConj e1 e2 => 1 + length_expr e1 + length_expr e2
+  | EBoolDisj e1 e2 => 1 + length_expr e1 + length_expr e2
+  | EBoolNeg e => 1 + length_expr e
+  | EInt _ => 1
+  | EMaxInt => 1
+  | EMinInt => 1
+  | EIntNeg e => 1 + length_expr e
+  | EIntAdd e1 e2 => 1 + length_expr e1 + length_expr e2
+  | EIntSub e1 e2 => 1 + length_expr e1 + length_expr e2
+  | EIntMul e1 e2 => 1 + length_expr e1 + length_expr e2
+  | EIntDiv e1 e2 => 1 + length_expr e1 + length_expr e2
+  | EIntMod e1 e2 => 1 + length_expr e1 + length_expr e2
+  | EChar _ => 1
+  | EString _ => 1
+  | EOpPhysEq e1 e2 => 1 + length_expr e1 + length_expr e2
+  | EOpEq e1 e2 => 1 + length_expr e1 + length_expr e2
+  | EOpNe e1 e2 => 1 + length_expr e1 + length_expr e2
+  | EOpLt e1 e2 => 1 + length_expr e1 + length_expr e2
+  | EOpLe e1 e2 => 1 + length_expr e1 + length_expr e2
+  | EOpGt e1 e2 => 1 + length_expr e1 + length_expr e2
+  | EOpGe e1 e2 => 1 + length_expr e1 + length_expr e2
   | ELet bs e =>
-      (* This is evaluated like a [match] construct with one branch. *)
-      try
-        (eval_bindings η bs)
-      (λ δ, η ← ret_concat δ η; eval η e)
-      match_failure
+      fold_left (fun acc b =>
+                   match b with
+                   | Binding _ e =>
+                       acc + length_expr e
+                   end) bs (1 + length_expr e)
   | ELetRec rbs e =>
-      (* Extend the environment with a mapping of each function name in [rbs]
-         to a suitable recursive closure; then, evaluate [e]. *)
-      let δ := eval_rec_bindings η rbs in
-      η ← ret_concat δ η;
-      eval η e
-  | ELetModule M me e =>
-      v ← eval_mexpr η me ;
-      let δ := EnvCons M v EnvNil in
-      η ← ret_concat δ η;
-      eval η e
-  | ELetOpen me e =>
-      δ ← as_struct (eval_mexpr η me) ;
-      η ← ret_concat δ η;
-      eval η e
-  | ESeq e1 e2 =>
-      _ ← eval η e1 ;
-      eval η e2
-  | EIfThen e e1 =>
-      b ← as_bool (eval η e) ;
-      if (b : bool) then eval η e1 else ok
-  | EIfThenElse e e1 e2 =>
-      b ← as_bool (eval η e) ;
-      if (b : bool) then eval η e1 else eval η e2
+      fold_left (fun acc rb =>
+                   match rb with
+                   | RecBinding _ afun =>
+                       match afun with
+                       | AnonFun _ e =>
+                           acc + length_expr e
+                       end
+                   end) rbs (1 + length_expr e)
+  | ELetModule _ _ e => 1 + length_expr e
+  | ELetOpen _ e => 1 + length_expr e
+  | ESeq e1 e2 => 1 + length_expr e1 + length_expr e2
+  | EIfThen e1 e2 => 1 + length_expr e1 + length_expr e2
+  | EIfThenElse e1 e2 e3 => 1 + length_expr e1 + length_expr e2 + length_expr e3
   | EMatch e bs =>
-      v ← eval η e ;
-      eval_match η v bs
-  | EWhile e body =>
-      b ← as_bool (eval η e) ;
-      if (b : bool) then
-        _ ← eval η body ;
-        stop CEval (η, EWhile e body)
-      else
-        ok
-  | EFor x e1 e2 e =>
-      (* The bounds are evaluated first. *)
-      '(i1, i2) ← par (as_int (eval η e1)) (as_int (eval η e2)) ;
-      (* Then, the loop is executed. *)
-      stop CLoop (η, x, i1, i2, e)
-  | EAssertFalse =>
-      assertion_failure
-  | EAssert e =>
-      (* OCaml runtime assertions are erased when a module is compiled with
-         the compiler flag [-noassert]; they are retained otherwise. We do not
-         wish to depend on this flag, so we make a non-deterministic choice:
-         either the runtime test is executed, or it is skipped. This forces
-         the user to prove that the program is safe in both scenarios. *)
-      let test : micro val :=
-        success ← as_bool (eval η e) ;
-        if (success : bool) then ok else assertion_failure
-      in
-      choose ok test
-  | ERef e =>
-      v ← eval η e ;
-      l ← stop CAlloc v ;
-      ret (VLoc l)
-  | ELoad e =>
-      l ← as_loc (eval η e) ;
-      stop CLoad l
-  | EStore e1 e2 =>
-      '(l, v) ← par (as_loc (eval η e1)) (eval η e2) ;
-      _ ← stop CStore (l, v) ;
-      ok
-  end
+      fold_left (fun acc b =>
+                   match b with
+                   | Branch _ e =>
+                       acc + length_expr e
+                   end) bs (1 + length_expr e)
+  | EWhile e1 e2 => 1 + length_expr e1 + length_expr e2
+  | EFor _ e1 e2 e3 => 1 + length_expr e1 + length_expr e2 + length_expr e3
+  | EAssertFalse => 1
+  | EAssert e => 1 + length_expr e
+  | ERef e => 1 + length_expr e
+  | ELoad e => 1 + length_expr e
+  | EStore e1 e2 => 1 + length_expr e1 + length_expr e2
+  end.
 
-(* ------------------------------------------------------------------------ *)
+Definition lt_expr e1 e2 :=
+  length_expr e1 < length_expr e2.
 
-(* [evals η es] evaluates the expressions [es] in the environment [η],
-   producing values [vs]. The expressions are evaluated in parallel. *)
+Lemma wf_length_expr :
+  well_founded lt_expr.
+Proof.
+  unfold lt_expr.
+  apply Inverse_Image.wf_inverse_image.
+  exact Nat.lt_wf_0.
+Qed.
 
-(* [evals] is used to evaluate tuples. *)
+Definition eval_bindings eval η bs :=
+  let f :=
+    fun b acc =>
+      match b with
+      | Binding p e =>
+          '(v, δ) ← par (eval η e) acc ;
+          extend δ p v
+      end
+  in
+  fold_right f (ret []) bs.
 
-with evals η es : micro vals :=
-  match es with
-  | ENil =>
-      ret VNil
-  | ECons e es =>
-      '(v, vs) ← par (eval η e) (evals η es) ;
-      ret (VCons v vs)
-  end
 
-(* ------------------------------------------------------------------------ *)
-
-(* [evalfs η fes] evaluates the expressions [fes] in the environment [η],
-   producing values [fvs]. The expressions are evaluated in parallel.
-
-   Each expression in the list [fes] and each value in the list [fvs]
-   is indexed with a record field. *)
-
-(* [evalfs] is used to evaluate record construction expressions. *)
-
-with evalfs η fes : micro env :=
-  match fes with
-  | FENil =>
-      ret EnvNil
-  | FECons f e fes =>
-      '(v, fvs) ← par (eval η e) (evalfs η fes) ;
-      ret (EnvCons f v fvs)
-  end
-
-(* ------------------------------------------------------------------------ *)
-
-(* [eval_bindings η bs] evaluates the bindings [bs] in the environment [η],
-   producing an environment fragment. *)
-
-(* [eval_bindings] is used to evaluate the [let/and] construct. *)
-
-(* A binding is a pair [p = e]. The expressions in the right-hand sides of the
-   bindings [bs] are evaluated in parallel. The values thus obtained are then
-   matched against the patterns in the left-hand sides. The pattern matching
-   process is sequential. *)
-
-(* If we chose to encode the multiple-let-and construct [let p_i = e_i in e]
-   as [let (p_i) = (e_i) in e], using a tuple and a single-let-and construct,
-   then [eval_bindings] would disappear. We prefer to avoid encodings. *)
-
-with eval_bindings η (bs : bindings) : micro env :=
-  match bs with
-  | BiNil =>
-      ret EnvNil
-  | BiCons (Binding p e) bs =>
-      (* Evaluate the expression [e], yielding a value [v]. In parallel,
-         evaluate the bindings [bs], yielding an environment fragment [δ]. *)
-      '(v, δ) ← par (eval η e) (eval_bindings η bs) ;
-      (* Match the value [v] against the pattern [p], extending [δ]. *)
-      extend δ p v
-  end
-
-(* ------------------------------------------------------------------------ *)
-
-(* [eval_match η v bs] evaluates [match v with bs] in the environment [η]. *)
-
-with eval_match η v bs : micro val :=
-  match bs with
-  | BrNil =>
-      (* A nonexhaustive [match] construct causes a hard failure. *)
-      (* Because the proof system forbids hard failures, the user of
-         the system will have to prove that this cannot happen, i.e.,
-         every case analysis is exhaustive. *)
-      match_failure()
-  | BrCons (Branch p e) bs =>
-      (* Match the value [v] against the pattern [p]. *)
-      try
-        (extend EnvNil p v)
-      (* Success: commit to this branch. Evaluate its body. *)
-      (λ δ, η ← ret_concat δ η; eval η e)
-      (* Soft failure: abandon this branch. Try the following branches. *)
-      (λ tt, eval_match η v bs)
-  end
-
-(* ------------------------------------------------------------------------ *)
-
-(* [eval_mexpr η me] evaluates the module expression [me] in environment [η],
-   yielding a value. *)
-
-with eval_mexpr η me : micro val :=
+Fixpoint length_mexpr me : nat :=
   match me with
-  | MUnsupported =>
-      unsupported_construct
-  | MPath π =>
+  | MUnsupported => 1
+  | MPath _ => 1
+  | MCoercion me _ => 1 + length_mexpr me
+  | MStruct items =>
+      let f :=
+        fun acc item =>
+          acc +
+          match item with
+          | ILet bs => 0
+          | ILetRec rbs => 0
+          | IModule _ me => length_mexpr me
+          | IOpen me => length_mexpr me
+          | IInclude me => length_mexpr me
+          end
+      in
+      fold_left f items 1
+  end.
+
+Definition lt_mexpr me1 me2 :=
+  length_mexpr me1 < length_mexpr me2.
+
+Lemma wf_length_mexpr :
+  well_founded lt_mexpr.
+Proof.
+  unfold lt_mexpr.
+  apply Inverse_Image.wf_inverse_image.
+  apply Nat.lt_wf_0.
+Qed.
+
+Program Fixpoint eval_mexpr eval η me : micro val :=
+  (* [eval_mexpr η me] evaluates the module expression [me] in environment [η],
+     yielding a value. *)
+  (match me as r return me = r -> micro val with
+  | MUnsupported => fun _ => unsupported_construct
+  | MPath π => fun _ =>
       (* A path is looked up in the environment [η]. *)
       lookup_path η π
-  | MStruct items =>
-      (* Beginning with an empty current structure, *)
-      let δ := EnvNil in
+  | MCoercion me c => fun _ =>
+      'v ← eval_mexpr eval η me ;
+       coerce c v
+  | MStruct items => fun Heq =>
       (* evaluate the structure items, yielding an environment [δ], *)
-      '(_, δ) ← eval_sitems (η, δ) items ;
-      (* and wrap it in a [VStruct] value. *)
-      ret (VStruct δ)
-  | MCoercion me c =>
-      v ← eval_mexpr η me ;
-      coerce c v
-  end
+      bind
+        (let eval_sitem :=
+           fun (acc : micro envs) item =>
+             match acc with
+             | ret ηδ =>
+                 let '(η, δ) := ηδ in
+                 match item as r' return item = r' -> micro envs with
+                 | ILet bs => fun Heq =>
+                     δ' ← eval_bindings eval η bs;
+                     ret_dconcat δ' (η, δ)
+                 | ILetRec rbs => fun Heq =>
+                     let δ' := eval_rec_bindings η rbs in
+                     ret_dconcat δ' (η, δ)
+                 | IModule m me' => fun Heq =>
+                     v ← eval_mexpr eval η me' ;
+                     ret_dconcat [(m, v)] (η, δ)
+                 | IOpen me' => fun Heq =>
+                     δ' ← as_struct (eval_mexpr eval η me') ;
+                     ret (δ' ++ η, δ)
+                 | IInclude me' => fun Heq =>
+                     δ' ← as_struct (eval_mexpr eval η me') ;
+                     ret (dconcat δ' (η, δ))
+                 end eq_refl
+             | _ => acc
+             end
+         in
+         fold_left eval_sitem items (ret (η, [])))
+        (fun '(_, δ) => ret (VStruct δ))
+   end) eq_refl.
 
-(* [eval_sitems ηδ items] evaluates the structure items [items] in the
-   double environment [ηδ], yielding an updated double environment. *)
+Next Obligation.
+  admit.
+Admitted.
 
-with eval_sitems ηδ items : micro envs :=
+Next Obligation.
+  admit.
+Admitted.
+
+Next Obligation.
+admit.
+Admitted.
+
+
+
+with eval_sitems eval ηδ items : micro envs :=
   match items with
-  | INil =>
-      ret ηδ
-  | ICons item items =>
-      (* Evaluate this item. *)
-      ηδ ← eval_sitem ηδ item ;
-      (* Evaluate the remaining items. *)
-      eval_sitems ηδ items
+  | [] => ret ηδ
+  | item :: items =>
+      let '(η, δ) := ηδ in
+      bind
+        ((fix eval_sitem η δ item :=
+            match item with
+            | ILet bs =>
+                δ' ← eval_bindings eval η bs;
+                ret_dconcat δ' (η, δ)
+            | ILetRec rbs =>
+                let δ' := eval_rec_bindings η rbs in
+                ret_dconcat δ' (η, δ)
+            | IModule m me =>
+                'v ← eval_mexpr eval η me ;
+                ret_dconcat [(m, v)] (η, δ)
+            | IOpen me =>
+                δ' ← as_struct (eval_mexpr eval η me) ;
+                ret (δ' ++ η, δ)
+            | IInclude me =>
+                δ' ← as_struct (eval_mexpr eval η me) ;
+                ret (dconcat δ' (η, δ))
+            end) η δ item)
+        (fun ηδ => eval_sitems eval ηδ items)
   end
+.
 
-(* [eval_sitem ηδ item] evaluates the structure item [item] in the
-   double environment [ηδ], yielding an updated double environment. *)
-
-with eval_sitem (ηδ : envs) item : micro envs :=
-  let '(η, δ) := ηδ in
+with eval_sitem eval (η δ : env) item : micro envs :=
   match item with
   | ILet bs =>
-      δ' ← eval_bindings η bs;
-      ret_dconcat δ' ηδ
+      δ' ← eval_bindings eval η bs;
+      ret_dconcat δ' (η, δ)
   | ILetRec rbs =>
       let δ' := eval_rec_bindings η rbs in
-      ret_dconcat δ' ηδ
+      ret_dconcat δ' (η, δ)
   | IModule m me =>
-      v ← eval_mexpr η me ;
-      let δ' := EnvCons m v EnvNil in
-      ret_dconcat δ' ηδ
+      'v ← eval_mexpr eval η me ;
+       ret_dconcat [(m, v)] (η, δ)
   | IOpen me =>
       (* The bindings contained in the structure denoted by the module
          expression [me] are used to extend [η] but not [δ]. This reflects
          the fact that these bindings become visible, but do not extend the
          current structure. *)
-      δ' ← as_struct (eval_mexpr η me) ;
-      ret (concat δ' η, δ)
+      'δ' ← as_struct (eval_mexpr eval η me) ;
+       ret (δ' ++ η, δ)
+  | IInclude me =>
+      δ' ← as_struct (eval_mexpr eval η me) ;
+      (* The bindings contained in the structure denoted by the module
+         expression [me] are used to extend both [η] and [δ]. *)
+      ret (dconcat δ' (η, δ))
+  end
+.
+
+Program Fixpoint eval η e {measure (length_expr e)} : micro val :=
+  match e with
+  | EUnsupported => unsupported_construct
+  | EChar c => ret (VChar c)
+  | EPath π =>
+      (* A path [π] is looked up in the environment [η]. *)
+      lookup_path η π
+  | EApp e1 e2 =>
+      (* The expressions [e1] and [e2] are evaluated in parallel. *)
+      '(v1, v2) ← par (eval η e1) (eval η e2) ;
+       call v1 v2
+  | ETuple es =>
+      (* The tuple components are evaluated in parallel. *)
+
+      (* [evals η es] evaluates the expressions [es] in the environment [η],
+         producing values [vs]. The expressions are evaluated in parallel. *)
+      'vs ← evals η es ;
+       ret (VTuple vs)
+  | ERecord fes =>
+      (* The record components are evaluated in parallel. *)
+
+      (* [evalfs η fes] evaluates the expressions [fes] in the environment [η],
+         producing values [fvs]. The expressions are evaluated in parallel. *)
+
+      (* Each expression in the list [fes] and each value in the list [fvs]
+         is indexed with a record field. *)
+      'fvs ← evalfs η fes ;
+      'fvs ← sort fvs ;
+       ret (VRecord fvs)
+  | ELet bs e =>
+      (* This is evaluated like a [match] construct with one branch. *)
+      try
+        (eval_bindings η bs)
+        (λ δ, η ← ret_concat δ η; eval η e)
+        match_failure
+  | EMatch e bs =>
+      'v ← eval η e ;
+       eval_match η v bs
+  | ELetModule M me e =>
+      'v ← eval_mexpr η me ;
+      'η ← ret_concat [(M, v)] η;
+       eval η e
+  | _ => unsupported_construct
+end
+
+with evals η es :=
+       let f :=
+         fun e acc =>
+           '(v, vs) ← par (eval η e) acc ;
+            ret (v :: vs)
+       in
+       fold_right f (ret []) es
+       (* match es with *)
+       (* | [] => *)
+       (*     ret [] *)
+       (* | e :: es => *)
+       (*     '(v, vs) ← par (eval η e) (evals η es) ; *)
+       (*      ret (v :: vs) *)
+       (* end *)
+
+with evalfs η fes :=
+       let f :=
+         fun fe acc =>
+           match fe with
+           | Fexpr f e =>
+               '(v, fvs) ← par (eval η e) (evalfs η fes) ;
+               ret ((f, v) :: fvs)
+           end
+       in
+       fold_right f (ret []) fes
+       (* match fes with *)
+       (* | [] => *)
+       (*     ret [] *)
+       (* | (Fexpr f e) :: fes => *)
+       (*     '(v, fvs) ← par (eval η e) (evalfs η fes) ; *)
+       (*      ret ((f, v) :: fvs) *)
+       (* end *)
+
+with eval_bindings eval η bs :=
+  let f :=
+    fun b acc =>
+      match b with
+      | Binding p e =>
+          '(v, δ) ← par (eval η e) acc ;
+          extend δ p v
+      end
+  in
+  fold_right f (ret []) bs
+  (*   match bs with *)
+  (*   | [] => *)
+  (*       ret [] *)
+  (*   | (Binding p e) :: bs => *)
+  (*       (* Evaluate the expression [e], yielding a value [v]. In parallel, *)
+  (*          evaluate the bindings [bs], yielding an environment fragment [δ]. *) *)
+  (*       '(v, δ) ← par (eval η e) (eval_bindings η bs) ; *)
+  (*        (* Match the value [v] against the pattern [p], extending [δ]. *) *)
+  (*        extend δ p v *)
+  (* end *)
+
+with eval_match η v (bs : list branch) {struct bs} : micro val :=
+  (* [eval_match η v bs] evaluates [match v with bs] in the environment [η]. *)
+  match bs with
+  | [] =>
+      (* A nonexhaustive [match] construct causes a hard failure. *)
+      (* Because the proof system forbids hard failures, the user of
+         the system will have to prove that this cannot happen, i.e.,
+         every case analysis is exhaustive. *)
+      match_failure()
+  | (Branch p e) :: bs =>
+      (* Match the value [v] against the pattern [p]. *)
+      try
+        (extend [] p v)
+        (* Success: commit to this branch. Evaluate its body. *)
+        (λ δ, η ← ret_concat δ η; eval η e)
+        (* Soft failure: abandon this branch. Try the following branches. *)
+        (λ tt, eval_match η v bs)
+  end
+
+with eval_mexpr η me {struct me} : micro val :=
+  (* [eval_mexpr η me] evaluates the module expression [me] in environment [η],
+     yielding a value. *)
+  match me with
+  | MUnsupported => unsupported_construct
+  | MPath π =>
+      (* A path is looked up in the environment [η]. *)
+      lookup_path η π
+  | MStruct items =>
+      (* Beginning with an empty current structure, *)
+      let δ := [] in
+      (* evaluate the structure items, yielding an environment [δ], *)
+      '(_, δ) ← eval_sitems (η, δ) items ;
+       (* and wrap it in a [VStruct] value. *)
+       ret (VStruct δ)
+  | MCoercion me c =>
+      'v ← eval_mexpr η me ;
+       coerce c v
+  end
+
+with eval_sitems ηδ items : micro envs :=
+  match items with
+  | [] => ret ηδ
+  | item :: items =>
+      let '(η, δ) := ηδ in
+      ηδ ← eval_sitem η δ item ;
+      (* Evaluate the remaining items. *)
+      eval_sitems ηδ items
+  end
+
+with eval_sitem (η δ : env) item : micro envs :=
+  match item with
+  | ILet bs =>
+      δ' ← eval_bindings η bs;
+      ret_dconcat δ' (η, δ)
+  | ILetRec rbs =>
+      let δ' := eval_rec_bindings η rbs in
+      ret_dconcat δ' (η, δ)
+  | IModule m me =>
+      'v ← eval_mexpr η me ;
+       ret_dconcat [(m, v)] (η, δ)
+  | IOpen me =>
+      (* The bindings contained in the structure denoted by the module
+         expression [me] are used to extend [η] but not [δ]. This reflects
+         the fact that these bindings become visible, but do not extend the
+         current structure. *)
+      'δ' ← as_struct (eval_mexpr η me) ;
+       ret (δ' ++ η, δ)
   | IInclude me =>
       δ' ← as_struct (eval_mexpr η me) ;
       (* The bindings contained in the structure denoted by the module
          expression [me] are used to extend both [η] and [δ]. *)
-      ret (dconcat δ' ηδ)
+      ret (dconcat δ' (η, δ))
   end
+.
+
+Equations eval η e : micro val by wf e lt_expr :=
+  eval η EUnsupported := unsupported_construct ;
+  eval η (EChar c) := ret (VChar c) ;
+  eval η (EPath π) :=
+    (* A path [π] is looked up in the environment [η]. *)
+    lookup_path η π ;
+  eval η (EAnonFun a) :=
+    (* The creation of a closure captures the environment [η]. *)
+    (* This environment is *not* trimmed so as to keep only the variables
+       that occur free in [a]. Indeed, in OCaml, due to [open], [include]
+       and other constructs, it is not easy to statically compute the set
+       of free variables of an expression. *)
+    ret (VClo η a) ;
+  eval η (EApp e1 e2) :=
+    (* The expressions [e1] and [e2] are evaluated in parallel. *)
+    '(v1, v2) ← par (eval η e1) (eval η e2) ;
+    call v1 v2 ;
+  eval η (ETuple es) :=
+    (* The tuple components are evaluated in parallel. *)
+
+    (* [evals η es] evaluates the expressions [es] in the environment [η],
+       producing values [vs]. The expressions are evaluated in parallel. *)
+    bind ((fix evals (η : env) es :=
+             match es with
+             | [] =>
+                 ret []
+             | e :: es =>
+                 '(v, vs) ← par (eval η e) (evals η es) ;
+               ret (v :: vs)
+             end) η es)
+      (λ vs : list val, ret (VTuple vs)) ;
+  eval η (EData c e) :=
+    v ← eval η e ;
+    ret (VData c v) ;
+  eval η (ERecord fes) :=
+    (* The record components are evaluated in parallel. *)
+
+    (* [evalfs η fes] evaluates the expressions [fes] in the environment [η],
+       producing values [fvs]. The expressions are evaluated in parallel. *)
+
+    (* Each expression in the list [fes] and each value in the list [fvs]
+       is indexed with a record field. *)
+    bind ((fix evalfs (η : env) fes : micro env :=
+             match fes with
+             | [] =>
+                 ret []
+             | (Fexpr f e) :: fes =>
+                 '(v, fvs) ← par (eval η e) (evalfs η fes) ;
+               ret ((f, v) :: fvs)
+             end) η fes)
+      (λ fvs : env, fvs ← sort fvs ;
+       ret (VRecord fvs)) ;
+  eval η (ERecordUpdate e fes) :=
+    (* The existing record and the new record components are evaluated in
+       parallel. *)
+    '(fvs, fvs') ← par
+      (as_record (eval η e))
+      ((fix evalfs (η : env) fes : micro env :=
+          match fes with
+          | [] =>
+              ret []
+          | (Fexpr f e) :: fes =>
+              '(v, fvs) ← par (eval η e) (evalfs η fes) ;
+            ret ((f, v) :: fvs)
+          end) η fes) ;
+      (* The new components override existing components by the same name. *)
+      fvs ← update fvs fvs' ;
+      fvs ← sort fvs ;
+      ret (VRecord fvs) ;
+  eval η (ERecordAccess e f) :=
+    fvs ← as_record (eval η e) ;
+    lookup_name fvs f ;
+  eval η (EBoolConj e1 e2) :=
+    b1 ← as_bool (eval η e1) ;
+    if (b1 : bool) then eval η e2 else ret VFalse ;
+  eval η (EString s) :=
+    ret (VString s) ;
+  eval η (EInt i) :=
+    (* An integer literal is interpreted as a machine integer. *)
+    (* We do not require this integer literal to lie within a certain
+       range; we project it into the range of machine integers. *)
+    ret (VInt (int.repr i)) ;
+  eval η EMaxInt :=
+    ret (VInt (int.repr int.max_signed)) ;
+  eval η EMinInt :=
+    ret (VInt (int.repr int.min_signed)) ;
+  eval η (EIntNeg e) :=
+    i ← as_int (eval η e) ;
+    ret (VInt (int.neg i)) ;
+  eval η (EIntAdd e1 e2) :=
+    '(i1, i2) ← par (as_int (eval η e1)) (as_int (eval η e2)) ;
+    ret (VInt (int.add i1 i2)) ;
+  eval η (EIntSub e1 e2) :=
+    '(i1, i2) ← par (as_int (eval η e1)) (as_int (eval η e2)) ;
+    ret (VInt (int.sub i1 i2)) ;
+  eval η (EIntMul e1 e2) :=
+    '(i1, i2) ← par (as_int (eval η e1)) (as_int (eval η e2)) ;
+    ret (VInt (int.mul i1 i2)) ;
+  eval η (EIntDiv e1 e2) :=
+    (* Signed division is used. *)
+    '(i1, i2) ← par (as_int (eval η e1)) (as_int (eval η e2)) ;
+    '() ← check_div_by_zero i2 ;
+    ret (VInt (int.divs i1 i2)) ;
+  eval η (EIntMod e1 e2) :=
+    (* Signed remainder is used. *)
+    '(i1, i2) ← par (as_int (eval η e1)) (as_int (eval η e2)) ;
+    '() ← check_div_by_zero i2 ;
+    ret (VInt (int.mods i1 i2)) ;
+  eval η (EOpPhysEq e1 e2) :=
+    '(v1, v2) ← par (eval η e1) (eval η e2) ;
+    b ← phys_eq_val v1 v2 ;
+    ret (VBool b) ;
+  eval η (EOpEq e1 e2) :=
+    '(v1, v2) ← par (eval η e1) (eval η e2) ;
+    b ← eq_val v1 v2 ;
+    ret (VBool b) ;
+  eval η (EOpNe e1 e2) :=
+    '(v1, v2) ← par (eval η e1) (eval η e2) ;
+    b ← ne_val v1 v2 ;
+    ret (VBool b) ;
+  eval η (EOpLt e1 e2) :=
+    '(v1, v2) ← par (eval η e1) (eval η e2) ;
+    b ← lt_val v1 v2 ;
+    ret (VBool b) ;
+  eval η (EOpLe e1 e2) :=
+    '(v1, v2) ← par (eval η e1) (eval η e2) ;
+    b ← le_val v1 v2 ;
+    ret (VBool b) ;
+  eval η (EOpGt e1 e2) :=
+    '(v1, v2) ← par (eval η e1) (eval η e2) ;
+    b ← gt_val v1 v2 ;
+    ret (VBool b) ;
+  eval η (EOpGe e1 e2) :=
+    '(v1, v2) ← par (eval η e1) (eval η e2) ;
+    b ← ge_val v1 v2 ;
+    ret (VBool b) ;
+  eval η (EBoolDisj e1 e2) :=
+    b1 ← as_bool (eval η e1) ;
+    if (b1 : bool) then ret VTrue else eval η e2 ;
+  eval η (EBoolNeg e) :=
+    b ← as_bool (eval η e) ;
+    ret (VBool (negb b)) ;
+  eval η (ELet bs e) :=
+      (* This is evaluated like a [match] construct with one branch. *)
+    try
+      (eval_bindings η bs)
+      (λ δ, η ← ret_concat δ η; eval η e)
+      match_failure ;
+  eval η (ELetRec rbs e) :=
+    (* Extend the environment with a mapping of each function name in [rbs]
+       to a suitable recursive closure; then, evaluate [e]. *)
+    let δ := eval_rec_bindings η rbs in
+    η ← ret_concat δ η;
+    eval η e ;
+  eval η (ELetModule M me e) :=
+    v ← eval_mexpr η me ;
+    η ← ret_concat [(M, v)] η;
+    eval η e ;
+  eval η (ELetOpen me e) :=
+    δ ← as_struct (eval_mexpr η me) ;
+    η ← ret_concat δ η;
+    eval η e ;
+  eval η (ESeq e1 e2) :=
+    _ ← eval η e1 ;
+    eval η e2 ;
+  eval η (EIfThen e e1) :=
+    b ← as_bool (eval η e) ;
+    if (b : bool) then eval η e1 else ok ;
+  eval η (EIfThenElse e e1 e2) :=
+    b ← as_bool (eval η e) ;
+    if (b : bool) then eval η e1 else eval η e2 ;
+  eval η (EMatch e bs) :=
+    v ← eval η e ;
+    eval_match η v bs ;
+  eval η (EWhile e body) :=
+    b ← as_bool (eval η e) ;
+    if (b : bool) then
+      _ ← eval η body ;
+      stop CEval (η, EWhile e body)
+    else
+      ok ;
+  eval η (EFor x e1 e2 e) :=
+    (* The bounds are evaluated first. *)
+    '(i1, i2) ← par (as_int (eval η e1)) (as_int (eval η e2)) ;
+    (* Then, the loop is executed. *)
+    stop CLoop (η, x, i1, i2, e) ;
+  eval η EAssertFalse := assertion_failure ;
+  eval η (EAssert e) =>
+    (* OCaml runtime assertions are erased when a module is compiled with
+       the compiler flag [-noassert]; they are retained otherwise. We do not
+       wish to depend on this flag, so we make a non-deterministic choice:
+       either the runtime test is executed, or it is skipped. This forces
+       the user to prove that the program is safe in both scenarios. *)
+    let test : micro val :=
+      success ← as_bool (eval η e) ;
+      if (success : bool) then ok else assertion_failure
+    in
+    choose ok test ;
+  eval η (ERef e) :=
+    v ← eval η e ;
+    l ← stop CAlloc v ;
+    ret (VLoc l) ;
+  eval η (ELoad e) :=
+    l ← as_loc (eval η e) ;
+    stop CLoad l ;
+  eval η (EStore e1 e2) :=
+    '(l, v) ← par (as_loc (eval η e1)) (eval η e2) ;
+    _ ← stop CStore (l, v) ;
+    ok;
+    
+where eval_bindings η (bs : list binding) : micro env :=
+  (* [eval_bindings η bs] evaluates the bindings [bs] in the environment [η],
+     producing an environment fragment. *)
+
+  (* [eval_bindings] is used to evaluate the [let/and] construct. *)
+
+  (* A binding is a pair [p = e]. The expressions in the right-hand sides of the
+     bindings [bs] are evaluated in parallel. The values thus obtained are then
+     matched against the patterns in the left-hand sides. The pattern matching
+     process is sequential. *)
+
+  (* If we chose to encode the multiple-let-and construct [let p_i = e_i in e]
+     as [let (p_i) = (e_i) in e], using a tuple and a single-let-and construct,
+     then [eval_bindings] would disappear. We prefer to avoid encodings. *)
+  eval_bindings η [] := ret [] ;
+  eval_bindings η ((Binding p e) :: bs) :=
+    (* Evaluate the expression [e], yielding a value [v]. In parallel,
+       evaluate the bindings [bs], yielding an environment fragment [δ]. *)
+    '(v, δ) ← par (eval η e) (eval_bindings η bs) ;
+    (* Match the value [v] against the pattern [p], extending [δ]. *)
+    extend δ p v ;
+
+where eval_match η v (bs : list branch) : micro val :=
+  (* [eval_match η v bs] evaluates [match v with bs] in the environment [η]. *)
+  
+  eval_match η v [] :=
+    (* A nonexhaustive [match] construct causes a hard failure. *)
+    (* Because the proof system forbids hard failures, the user of
+       the system will have to prove that this cannot happen, i.e.,
+       every case analysis is exhaustive. *)
+    match_failure() ;
+  eval_match η v ((Branch p e) :: bs) :=
+    (* Match the value [v] against the pattern [p]. *)
+    try
+      (extend [] p v)
+      (* Success: commit to this branch. Evaluate its body. *)
+      (λ δ, η ← ret_concat δ η; eval η e)
+      (* Soft failure: abandon this branch. Try the following branches. *)
+      (λ tt, eval_match η v bs) ;
+
+where eval_mexpr η me : micro val :=
+  (* [eval_mexpr η me] evaluates the module expression [me] in environment [η],
+     yielding a value. *)
+
+  eval_mexpr η MUnsupported := unsupported_construct ;
+  eval_mexpr η (MPath π) :=
+    (* A path is looked up in the environment [η]. *)
+    lookup_path η π ;
+  eval_mexpr η (MStruct items) :=
+    (* Beginning with an empty current structure, *)
+    let δ := [] in
+    (* evaluate the structure items, yielding an environment [δ], *)
+    '(_, δ) ← eval_sitems (η, δ) items ;
+    (* and wrap it in a [VStruct] value. *)
+    ret (VStruct δ) ;
+  eval_mexpr η (MCoercion me c) :=
+    v ← eval_mexpr η me ;
+    coerce c v ;
+
+(* [eval_sitems ηδ items] evaluates the structure items [items] in the
+   double environment [ηδ], yielding an updated double environment. *)
+
+with eval_sitems ηδ items : micro envs :=
+  eval_sitems ηδ [] := ret ηδ ;
+  eval_sitems ηδ (item :: items) :=
+    (* Evaluate this item. *)
+    let '(η, δ) := ηδ in
+    ηδ ← eval_sitem η δ item ;
+    (* Evaluate the remaining items. *)
+    eval_sitems ηδ items ;
+
+(* [eval_sitem ηδ item] evaluates the structure item [item] in the
+   double environment [ηδ], yielding an updated double environment. *)
+
+where eval_sitem (η δ : env) item : micro envs :=
+  eval_sitem η δ (ILet bs) :=
+    δ' ← eval_bindings η bs;
+    ret_dconcat δ' (η, δ) ;
+  eval_sitem η δ (ILetRec rbs) :=  
+    let δ' := eval_rec_bindings η rbs in
+    ret_dconcat δ' (η, δ) ;
+  eval_sitem η δ (IModule m me) :=
+    v ← eval_mexpr η me ;
+    ret_dconcat [(m, v)] (η, δ) ;
+  eval_sitem η δ (IOpen me) :=
+    (* The bindings contained in the structure denoted by the module
+       expression [me] are used to extend [η] but not [δ]. This reflects
+       the fact that these bindings become visible, but do not extend the
+       current structure. *)
+    δ' ← as_struct (eval_mexpr η me) ;
+    ret (δ' ++ η, δ) ;
+  eval_sitem η δ (IInclude me) :=
+    δ' ← as_struct (eval_mexpr η me) ;
+    (* The bindings contained in the structure denoted by the module
+       expression [me] are used to extend both [η] and [δ]. *)
+    ret (dconcat δ' (η, δ))
 
 .
 
